CSE: add recognition of some combined operators, conditions, and addressing modes (cf. CombineOp.v) Memory model: cleaning up Memdata Inlining and new Constprop: updated for ARM.
git-svn-id: https://yquem.inria.fr/compcert/svn/compcert/trunk@1902 fca1b0fc-160b-0410-b1d3-a4f43f01ea2e

arm/Unusedglob1.ml
@@ -26,7 +26,7 @@ let referenced_instr = function
   | Pbsymb(s, _) -> [s]
   | Pblsymb(s, _) -> [s]
   | Ploadsymbol(_, s, _) -> [s]
-  | Pbuiltin ef -> referenced_builtin ef
+  | Pbuiltin(ef, _, _) -> referenced_builtin ef
   | _ -> []
 
 let code_of_function f = f.fn_code
