arm/CombineOpproof.v
@@ -1,0 +1,127 @@
+(* *********************************************************************)
+(*                                                                     *)
+(*              The Compcert verified compiler                         *)
+(*                                                                     *)
+(*          Xavier Leroy, INRIA Paris-Rocquencourt                     *)
+(*                                                                     *)
+(*  Copyright Institut National de Recherche en Informatique et en     *)
+(*  Automatique.  All rights reserved.  This file is distributed       *)
+(*  under the terms of the INRIA Non-Commercial License Agreement.     *)
+(*                                                                     *)
+(* *********************************************************************)
+
+(** Recognition of combined operations, addressing modes and conditions 
+  during the [CSE] phase. *)
+
+Require Import Coqlib.
+Require Import AST.
+Require Import Integers.
+Require Import Values.
+Require Import Memory.
+Require Import Op.
+Require Import Registers.
+Require Import RTL.
+Require Import CombineOp.
+Require Import CSE.
+
+Section COMBINE.
+
+Variable ge: genv.
+Variable sp: val.
+Variable m: mem.
+Variable get: valnum -> option rhs.
+Variable valu: valnum -> val.
+Hypothesis get_sound: forall v rhs, get v = Some rhs -> equation_holds valu ge sp m v rhs.
+
+Lemma combine_compimm_ne_0_sound:
+  forall x cond args,
+  combine_compimm_ne_0 get x = Some(cond, args) ->
+  eval_condition cond (map valu args) m = Val.cmp_bool Cne (valu x) (Vint Int.zero) /\
+  eval_condition cond (map valu args) m = Val.cmpu_bool (Mem.valid_pointer m) Cne (valu x) (Vint Int.zero).
+Proof.
+  intros until args. functional induction (combine_compimm_ne_0 get x); intros EQ; inv EQ.
+  (* of cmp *)
+  exploit get_sound; eauto. unfold equation_holds. simpl. intro EQ; inv EQ. 
+  destruct (eval_condition cond (map valu args) m); simpl; auto. destruct b; auto.
+Qed.
+
+Lemma combine_compimm_eq_0_sound:
+  forall x cond args,
+  combine_compimm_eq_0 get x = Some(cond, args) ->
+  eval_condition cond (map valu args) m = Val.cmp_bool Ceq (valu x) (Vint Int.zero) /\
+  eval_condition cond (map valu args) m = Val.cmpu_bool (Mem.valid_pointer m) Ceq (valu x) (Vint Int.zero).
+Proof.
+  intros until args. functional induction (combine_compimm_eq_0 get x); intros EQ; inv EQ.
+  (* of cmp *)
+  exploit get_sound; eauto. unfold equation_holds. simpl. intro EQ; inv EQ. 
+  rewrite eval_negate_condition. 
+  destruct (eval_condition c (map valu args) m); simpl; auto. destruct b; auto.
+Qed.
+
+Theorem combine_cond_sound:
+  forall cond args cond' args',
+  combine_cond get cond args = Some(cond', args') ->
+  eval_condition cond' (map valu args') m = eval_condition cond (map valu args) m.
+Proof.
+  intros. functional inversion H; subst.
+  (* compimm ne zero *)
+  simpl; eapply combine_compimm_ne_0_sound; eauto.
+  (* compimm eq zero *)
+  simpl; eapply combine_compimm_eq_0_sound; eauto.
+  (* compuimm ne zero *)
+  simpl; eapply combine_compimm_ne_0_sound; eauto.
+  (* compuimm eq zero *)
+  simpl; eapply combine_compimm_eq_0_sound; eauto.
+Qed.
+
+Theorem combine_addr_sound:
+  forall addr args addr' args',
+  combine_addr get addr args = Some(addr', args') ->
+  eval_addressing ge sp addr' (map valu args') = eval_addressing ge sp addr (map valu args).
+Proof.
+  intros. functional inversion H; subst.
+  (* indexed - addimm *)
+  exploit get_sound; eauto. unfold equation_holds; simpl; intro EQ. FuncInv.
+  rewrite <- H0. rewrite Val.add_assoc. auto. 
+  (* indexed 0 - add *)
+  exploit get_sound; eauto. unfold equation_holds; simpl; intro EQ. FuncInv.
+  rewrite <- H0. destruct v; destruct v0; simpl; auto; rewrite Int.add_zero; auto.
+  (* indexed 0 - addshift *)
+  exploit get_sound; eauto. unfold equation_holds; simpl; intro EQ. FuncInv.
+  rewrite <- H0. destruct v; destruct (eval_shift s v0); simpl; auto; rewrite Int.add_zero; auto.
+Qed.
+
+Theorem combine_op_sound:
+  forall op args op' args',
+  combine_op get op args = Some(op', args') ->
+  eval_operation ge sp op' (map valu args') m = eval_operation ge sp op (map valu args) m.
+Proof.
+  intros. functional inversion H; subst.
+(* addimm - addimm *)
+  exploit get_sound; eauto. unfold equation_holds; simpl; intros. FuncInv.
+  rewrite <- H1. rewrite Val.add_assoc. auto.
+(* addimm - subimm *)
+Opaque Val.sub.
+  exploit get_sound; eauto. unfold equation_holds; simpl; intros. FuncInv.
+  rewrite <- H1. change (Vint (Int.add m0 n)) with (Val.add (Vint m0) (Vint n)).
+  rewrite Val.sub_add_l. auto.
+(* subimm - addimm *)
+  exploit get_sound; eauto. unfold equation_holds; simpl; intros. FuncInv.
+  rewrite <- H1.
+Transparent Val.sub.
+  destruct v; simpl; auto. repeat rewrite Int.sub_add_opp. rewrite Int.add_assoc.
+  rewrite Int.neg_add_distr. decEq. decEq. decEq. apply Int.add_commut.
+(* andimm - andimm *)
+  exploit get_sound; eauto. unfold equation_holds; simpl; intros. FuncInv.
+  rewrite <- H1. rewrite Val.and_assoc. auto.
+(* orimm - orimm *)
+  exploit get_sound; eauto. unfold equation_holds; simpl; intros. FuncInv.
+  rewrite <- H1. rewrite Val.or_assoc. auto.
+(* xorimm - xorimm *)
+  exploit get_sound; eauto. unfold equation_holds; simpl; intros. FuncInv.
+  rewrite <- H1. rewrite Val.xor_assoc. auto.
+(* cmp *)
+  simpl. decEq; decEq. eapply combine_cond_sound; eauto.
+Qed.
+
+End COMBINE.
